formal/fstar/run_compile.sh
@@ -1,0 +1,9 @@
+#!/usr/bin/env bash
+set -uo pipefail
+cd /home/user/factoidal/formal/fstar
+eval $(opam env --switch=fstar)
+rm -f COMPILE_DONE compile.log
+RC=0
+./build-ocaml.sh compile > compile.log 2>&1 || RC=$?
+echo "COMPILE_RC=$RC" >> compile.log
+touch COMPILE_DONE
